\subsection{Strong subadditivity}\label{StrSubAdd}
For any quantum systems $A, B, C,$ the inequalities
\begin{align*}
H(A)+H(C) \leq H(AB)+H(BC) \\
H(ABC)+H(C) \leq H(AC)+H(BC)
\end{align*}
hold.

\emph{Proof:} Define a function $T(\rho ^{ABC})$ of density operators on the system ABC,
\begin{align*}
T(\rho ^{ABC}) &\equiv H(A)+H(C)-H(AB)-H(BC) \\
&= -H(B|A) -H(B|C) .
\end{align*}
  From the concavity of the conditional entropy we see that $T(\rho ^{ABC})$ is a convex function of $\rho ^{ABC}$ of density operators on the system $ABC$.
Let $\rho ^{ABC} = \sum_ip_i|i \rangle \langle i|$ be a spectral decomposition of $\rho ^{ABC}$.

  From the convexity of $T$, $T(\rho ^{ABC}) \leq \sum_ip_iT(|i \rangle \langle i|)$. But $T(|i \rangle \langle i|)=0$ as for a pure state $H(AB)=H(C)$ and $H(BC)=H(A)$. It follows that $T(\rho ^{ABC}) \leq 0$, and thus
\begin{align*}
H(A)+H(C)-H(AB)-H(BC) \leq 0,
\end{align*}
which is the first inequality we set out to prove.

  To obtain the second inuquality, introduce an auxiliary system $R$ purifying the system $ABC$. Then using the just-proved inuquality we have
\begin{align*}
H(R)+H(C) \leq H(RB)+H(BC).
\end{align*}
  Since ABCR is a pure state, $H(R)=H(ABC)$ and $H(RB)=H(AC)$, so becomes
\begin{align*}
H(ABC)+H(C) \leq H(AC)+H(BC).
\end{align*}
Therefore, we finish the proof.